Add determinism for all semantics

CE_FBOS.v
@@ -75,8 +75,9 @@ Inductive ResultListType : Type :=
 | LTimeout
 | LFailure.
 
+Require Import FunInd.
 
-Fixpoint eval_fbos_expr (env : Environment) (id : nat) (exp : Expression) (eff : SideEffectList)  (clock : nat) : 
+Fixpoint eval_fbos_expr (env : Environment) (id : nat) (exp : Expression) (eff : SideEffectList)  (clock : nat) {struct clock} : 
   ResultType :=
 match clock with
 | 0 => Timeout
@@ -227,6 +228,10 @@ match clock with
   end
 end
 .
+
+(* Functional Scheme div2_ind := Induction for eval_fbos_expr Sort Set.
+TODO: report todo error here
+ *)
 
 Example exp1 := ELet "X"%string (ELet "X"%string (ELit (Integer 5)) (EVar "X"%string)) (ELet "X"%string (ELet "X"%string (ELit (Integer 5)) (EVar "X"%string)) (ELet "X"%string (ELet "X"%string (ELit (Integer 5)) (EVar "X"%string)) (ELet "X"%string (ELet "X"%string (ELit (Integer 5)) (EVar "X"%string)) (ELet "X"%string (ELet "X"%string (ELit (Integer 5)) (EVar "X"%string)) (ELet "X"%string (ELet "X"%string (ELit (Integer 5)) (EVar "X"%string)) (ELet "X"%string (ELet "X"%string (ELit (Integer 5)) (EVar "X"%string)) (ELet "X"%string (ELet "X"%string (ELit (Integer 5)) (EVar "X"%string)) (ELet "X"%string (ELet "X"%string (ELit (Integer 5)) (EVar "X"%string)) ( ELet "X"%string (ELet "X"%string (ELit (Integer 5)) (EVar "X"%string)) (ELet "X"%string (ELet "X"%string (ELit (Integer 5)) (EVar "X"%string)) (ELet "X"%string (ELet "X"%string (ELit (Integer 5)) (EVar "X"%string)) (ELet "X"%string (ELet "X"%string (ELit (Integer 5)) (EVar "X"%string)) (ELet "X"%string (ELet "X"%string (ELit (Integer 5)) (EVar "X"%string)) (ELet "X"%string (ELet "X"%string (ELit (Integer 5)) (EVar "X"%string)) (ELet "X"%string (ELet "X"%string (ELit (Integer 5)) (EVar "X"%string)) (ELet "X"%string (ELet "X"%string (ELit (Integer 5)) (EVar "X"%string)) (ELet "X"%string (ELet "X"%string (ELit (Integer 5)) (EVar "X"%string)) ( ELet "X"%string (ELet "X"%string (ELit (Integer 5)) (EVar "X"%string)) (ELet "X"%string (ELet "X"%string (ELit (Integer 5)) (EVar "X"%string)) (ELet "X"%string (ELet "X"%string (ELit (Integer 5)) (EVar "X"%string)) (ELet "X"%string (ELet "X"%string (ELit (Integer 5)) (EVar "X"%string)) (ELet "X"%string (ELet "X"%string (ELit (Integer 5)) (EVar "X"%string)) (ELet "X"%string (ELet "X"%string (ELit (Integer 5)) (EVar "X"%string)) (ELet "X"%string (ELet "X"%string (ELit (Integer 5)) (EVar "X"%string)) (ELet "X"%string (ELet "X"%string (ELit (Integer 5)) (EVar "X"%string)) (ELet "X"%string (ELet "X"%string (ELit (Integer 5)) (EVar "X"%string)) ( ELet "X"%string (ELet "X"%string (ELit (Integer 5)) (EVar "X"%string)) (ELet "X"%string (ELet "X"%string (ELit (Integer 5)) (EVar "X"%string)) (ELet "X"%string (ELet "X"%string (ELit (Integer 5)) (EVar "X"%string)) (ELet "X"%string (ELet "X"%string (ELit (Integer 5)) (EVar "X"%string)) (ELet "X"%string (ELet "X"%string (ELit (Integer 5)) (EVar "X"%string)) (ELet "X"%string (ELet "X"%string (ELit (Integer 5)) (EVar "X"%string)) (ELet "X"%string (ELet "Y"%string (ELit (Integer 5)) (EVar "Y"%string)) (ELet "X"%string (ELet "X"%string (ELit (Integer 5)) (EVar "X"%string)) (ELet "X"%string (ELet "X"%string (ELit (Integer 5)) (EVar "X"%string)) (ECall "+"%string [EVar "X"%string; EVar "X"%string])))))))))))))))))))))))))))))))))))).
 
