CE_NOS.v
@@ -520,7 +520,7 @@ Proof.
       apply alma. assumption.
   }
 Qed.
-
+*)
 Section Tactic.
 
 Theorem length_succ {B : Type} (a2 : B) (n : nat) (l2 : list B):
@@ -575,7 +575,7 @@ match goal with
 | |- | ?env, ?id, EVar ?v, ?eff | -e> | ?id', ?res, ?eff'| => finishing_tactic
 | |- | ?env, ?id, EFunId ?fid, ?eff | -e> | ?id', ?res, ?eff'| => finishing_tactic
 | |- | ?env, ?id, EFun ?pl ?b, ?eff | -e> | ?id', ?res, ?eff'| => finishing_tactic
-| |- | ?env, ?id, ETuple ?l, ?eff | -e> | ?id', ?res, ?eff'| =>
+(* | |- | ?env, ?id, ETuple ?l, ?eff | -e> | ?id', ?res, ?eff'| =>
      (* (apply quick_tuple_eval; simpl; reflexivity)
      + *)
      (eapply eval_tuple;
@@ -616,7 +616,7 @@ match goal with
       | _ => idtac
       end;
       try(simpl;reflexivity);
-      solve_inners)
+      solve_inners) *)
 | |- | ?env, ?id, ECall _ ?l, ?eff | -e> | ?id', ?res, ?eff'| =>
      (eapply eval_call;
      unfold_list2;
@@ -702,7 +702,7 @@ match goal with
 | |- | _, _, _, _ | -e> | _, _, _ | => tryif solve then idtac else fail 1
 | _ => idtac
 end
-with
+(* with
 case_solver num :=
   tryif 
     eapply eval_case with (i := num);
@@ -747,7 +747,7 @@ tuple_exception_solver num :=
     idtac
   else
     tuple_exception_solver (S num)
-  end
+  end *)
 with
 app_param_exception_solver num :=
   match goal with
@@ -798,4 +798,776 @@ Proof.
   end. solve. simpl. solve.
 Qed.
 
-End Tactic. *)
+End Tactic.
+
+
+Section determinism_proof.
+
+Ltac empty_list_in_hypo :=
+match goal with
+| [H : 0 = length _ |- _ ] => apply eq_sym, length_zero_iff_nil in H
+| [H : length _ = 0 |- _ ] => apply length_zero_iff_nil in H
+| _ => idtac
+end.
+
+Ltac single_unfold_list :=
+match goal with
+| [ Hyp : Datatypes.length ?l = 0 |- _] => apply length_zero_iff_nil in Hyp; subst
+| [ Hyp : 0 = Datatypes.length ?l |- _] => apply eq_sym, length_zero_iff_nil in Hyp; subst
+| [ Hyp : Datatypes.length ?l = S ?n |- _] => symmetry in Hyp; single_unfold_list
+| [ Hyp : S ?n = Datatypes.length ?l |- _] => 
+   pose (element_exist _ _ Hyp);
+   match goal with
+   | [H' : exists x l', _ = x::l' |- _] => 
+     inversion H';
+     match goal with
+     | [H'' : exists l', _ = ?x::l' |- _] => inversion H''; subst; simpl in Hyp; inversion Hyp
+     end
+   end
+end
+.
+
+Lemma restrict_helper {env : Environment} {eff1 : SideEffectList} {exps : list Expression} 
+    (a : Expression) (x1 : SideEffectList) (x6 : list SideEffectList) (x0 : Value) 
+    (x3 : list Value) (id' : nat) (ids : list nat) (id : nat):
+(forall i : nat,
+    i < Datatypes.length (a :: exps) ->
+    | env, nth_def (id'::ids) id 0 i, nth i (a :: exps) ErrorExp, nth_def (x1 :: x6) eff1 [] i | -e>
+    | nth_def (id'::ids) id 0 (S i), inl (nth i (x0 :: x3) ErrorValue), nth_def (x1 :: x6) eff1 [] (S i) |)
+->
+forall i : nat,
+    i < Datatypes.length exps ->
+    | env, nth_def ids id' 0 i, nth i exps ErrorExp, nth_def x6 x1 [] i | -e>
+    | nth_def ids id' 0 (S i), inl (nth i x3 ErrorValue), nth_def x6 x1 [] (S i) |
+.
+Proof.
+  intros.
+  assert (S i < Datatypes.length (a :: exps)) as A1.
+  { simpl. lia. } pose (E := H (S i) A1). 
+  (* pose (P1 := @concatn_app eff1 x1 x6 i).
+  pose (P2 := @concatn_app eff1 x1 x6 (S i)).
+  rewrite P1, P2 in E. *) simpl in E. simpl. unfold nth_def. exact E.
+Qed.
+
+Lemma list_equality {env : Environment} {exps : list Expression} {eff1 : SideEffectList} : 
+forall vals vals0 : list Value, forall eff eff4 : list SideEffectList,
+forall id ids ids0,
+  (forall i : nat,
+     i < Datatypes.length exps ->
+     | env, nth_def ids id 0 i, nth i exps ErrorExp, nth_def eff eff1 [] i | 
+     -e> 
+     | nth_def ids id 0 (S i), inl (nth i vals ErrorValue), nth_def eff eff1 [] (S i) |)
+->
+(forall i : nat,
+     i < Datatypes.length exps ->
+     forall (v2 : Value + Exception) (eff'' : SideEffectList) (id'' : nat),
+     | env, nth_def ids id 0 i, nth i exps ErrorExp, nth_def eff eff1 [] i |
+     -e>
+     | id'', v2, eff'' | ->
+     inl (nth i vals ErrorValue) = v2 /\ nth_def eff eff1 [] (S i) = eff'' /\ nth_def ids id 0 (S i) = id'')
+->
+(forall i : nat,
+     i < Datatypes.length exps ->
+     | env, nth_def ids0 id 0 i, nth i exps ErrorExp, nth_def eff4 eff1 [] i |
+     -e> 
+     | nth_def ids0 id 0 (S i), inl (nth i vals0 ErrorValue), nth_def eff4 eff1 [] (S i) |)
+->
+Datatypes.length exps = Datatypes.length vals0
+->
+Datatypes.length exps = Datatypes.length eff4
+->
+Datatypes.length exps = Datatypes.length vals
+->
+Datatypes.length exps = Datatypes.length eff
+->
+length exps = length ids
+->
+length exps = length ids0
+->
+eff = eff4 /\ vals = vals0 /\ ids = ids0.
+Proof.
+  generalize dependent eff1. induction exps.
+  * intros. simpl in H3, H2, H4, H5, H6, H7.
+    repeat (empty_list_in_hypo).
+    subst. auto.
+  * intros. inversion H3. inversion H2. inversion H4. inversion H5. inversion H6. inversion H7.
+  
+  (* first elements are the same *)
+    single_unfold_list. single_unfold_list.
+    single_unfold_list. single_unfold_list.
+    single_unfold_list. single_unfold_list.
+    pose (P1 := H1 0 list_length).
+    pose (P2 := H0 0 list_length (inl x7) (nth_def (x9 :: x10) eff1 [] 1) x).
+    pose (P3 := P2 P1). inversion P3. inversion H25. inversion H27. simpl in H28. simpl in H30.
+    subst.
+  (* remaining lists are the same *)
+
+  (* These three asserts ensure, that if something states for every element in 
+    a (b::l) list, then it states for every element in l too*)
+    assert (
+      (forall i : nat,
+    i < Datatypes.length exps ->
+    | env, nth_def x2 x 0 i, nth i exps ErrorExp, nth_def x4 x9 [] i | -e> 
+    | nth_def x2 x 0 (S i), inl (nth i x6 ErrorValue),
+    nth_def x4 x9 [] (S i) |)
+    ).
+    {
+      intros. pose (P4 := restrict_helper a _ _ _ _ _ _ _ H i H28). assumption.
+    }
+    assert (
+      (forall i : nat,
+      i < Datatypes.length exps ->
+      forall (v2 : Value + Exception) (eff'' : SideEffectList) (id'' : nat),
+      | env, nth_def x2 x 0 i, nth i exps ErrorExp, nth_def x4 x9 [] i | -e> | id'', v2, eff'' | ->
+      inl (nth i x6 ErrorValue) = v2 /\ nth_def x4 x9 [] (S i) = eff'' /\ nth_def x2 x 0 (S i) = id'')
+    ).
+    {
+      intros. assert (S i < Datatypes.length (a::exps)). { simpl. lia. } 
+      pose (P4 := H0 (S i) H31 v2 eff'' id''). simpl nth in P4. exact (P4 H30).
+    }
+    assert (
+     (forall i : nat,
+    i < Datatypes.length exps ->
+    | env, nth_def x0 x 0 i, nth i exps ErrorExp, nth_def x10 x9 [] i | -e>
+    | nth_def x0 x 0 (S i), inl (nth i x8 ErrorValue),
+    nth_def x10 x9 [] (S i) |)
+    ).
+    {
+      intros. assert (S i < Datatypes.length (a :: exps)). { simpl. lia. } 
+      pose (P4 := H1 (S i) H31). simpl nth in P4. assumption.
+    }
+    (* simpl list lengths *)
+    inversion H10. inversion H11. inversion H12. inversion H13. inversion H14.
+    pose (IH := IHexps x9 x6 x8 x4 x10 x x2 x0 H28 H29 H30 H32 H26 H33 H34 H35 H36). 
+    inversion IH. inversion H37. subst. auto.
+Qed.
+
+Lemma firstn_eq {env : Environment} {eff : list SideEffectList} : 
+forall (eff5 : list SideEffectList) (exps : list Expression) (vals vals0 : list Value) 
+   (eff1 : SideEffectList) (ids ids0 : list nat) (id id'' : nat) ex eff3,
+length exps = length vals ->
+Datatypes.length exps = Datatypes.length eff
+->
+Datatypes.length eff5 = Datatypes.length vals0
+->
+Datatypes.length vals0 < Datatypes.length exps 
+->
+length exps = length ids
+->
+length ids0 = length vals0
+->
+(forall i : nat,
+     i < Datatypes.length exps ->
+     forall (v2 : Value + Exception) (eff'' : SideEffectList) (id'' : nat),
+     | env, nth_def ids id 0 i, nth i exps ErrorExp, nth_def eff eff1 [] i | -e> | id'', v2, eff'' | ->
+     inl (nth i vals ErrorValue) = v2 /\ nth_def eff eff1 [] (S i) = eff'' /\ nth_def ids id 0 (S i) = id'')
+->
+(forall j : nat,
+     j < Datatypes.length vals0 ->
+     | env, nth_def ids0 id 0 j, nth j exps ErrorExp, nth_def eff5 eff1 [] j | -e>
+     | nth_def ids0 id 0 (S j), inl (nth j vals0 ErrorValue),
+     nth_def eff5 eff1 [] (S j) |)
+->
+| env, last ids0 id, nth (Datatypes.length vals0) exps ErrorExp,
+      last eff5 eff1 | -e> | id'', inr ex,
+      eff3 |
+->
+False.
+Proof.
+  induction eff.
+  * intros. inversion H0. rewrite H9 in H2. inversion H2.
+  * intros. destruct eff5.
+    - inversion H1. simpl in H1. apply eq_sym, length_zero_iff_nil in H1. subst.
+      simpl in H4.
+      apply length_zero_iff_nil in H4. subst. simpl in H0. rewrite H0 in H5.
+      pose (P := H5 0 (Nat.lt_0_succ _) _ _ _ H7). destruct P. inversion H1.
+    - inversion H1. simpl.
+    (* first elements *)
+      inversion H0.
+      assert (0 < length exps). { lia. }
+      assert (0 < length vals0). { lia. }
+      assert (0 < length ids0). { lia. }
+      simpl in H0, H1.
+      (* single_unfold_list H1. *)
+      assert (Datatypes.length exps = S (Datatypes.length eff)) as Helper. { auto. }
+      assert (Datatypes.length ids0 = Datatypes.length vals0) as Helper2. { auto. }
+      assert (Datatypes.length exps = Datatypes.length ids) as Helper3. { auto. }
+      pose (EE1 := element_exist _ _ (eq_sym H10)).
+      pose (EE2 := element_exist _ _ H1).
+      rewrite H in H0.
+      pose (EE3 := element_exist _ _ (eq_sym H0)).
+      rewrite <- H1 in H4. rewrite H10 in H3.
+      pose (EE4 := element_exist _ _ H3).
+      pose (EE5 := element_exist _ _ (eq_sym H4)).
+      inversion EE1 as [e]. inversion EE2 as [v]. inversion EE3 as [v'].
+      inversion EE4 as [id0']. inversion EE5 as [id0'']. 
+      inversion H13. inversion H14. inversion H15. inversion H16. inversion H17. subst.
+      pose (P0 := H6 0 H11).
+      pose (P1 := H5 0 H8 (inl v) (s)).
+      pose (P2 := P1 _ P0). destruct P2. destruct H18, H19. simpl in H18, H19. subst.
+    (* other elements *)
+      inversion H1.
+      eapply IHeff with (exps := x) (vals := x1) (vals0 := x0) (eff1 := s)
+                      (ids := x2) (ids0 := x3) (id := id0'') (eff5 := eff5); auto.
+        + intuition.
+        + intros. assert (S i < Datatypes.length (e :: x)). { simpl. lia. }
+          pose (A := H5 (S i) H21 v2 eff''). simpl in A, H20.
+          pose (B := A _ H20). assumption.
+        + intros. assert (S j < Datatypes.length (v :: x0)). { lia. } 
+          pose (A := H6 (S j) H20). exact A.
+        + rewrite <- last_element_equal, <- last_element_equal in H7. exact H7.
+Qed.
+
+(** Side effect equality until the ith element using concatn *)
+Lemma eff_until_i {env : Environment} {eff : list SideEffectList} : 
+forall (eff5 : list SideEffectList) {exps : list Expression} (vals vals0 : list Value) 
+   (eff1 : SideEffectList) (ids ids0 : list nat) (id id'' : nat) ex  eff3,
+length exps = length vals ->
+Datatypes.length exps = Datatypes.length eff
+->
+Datatypes.length eff5 = Datatypes.length vals0
+->
+Datatypes.length vals0 < Datatypes.length exps 
+->
+length exps = length ids
+->
+length ids0 = length vals0
+->
+(forall i : nat,
+     i < Datatypes.length exps ->
+     forall (v2 : Value + Exception) (eff'' : SideEffectList) (id'' : nat),
+     | env, nth_def ids id 0 i, nth i exps ErrorExp, nth_def eff eff1 [] i | -e> | id'', v2, eff'' | ->
+     inl (nth i vals ErrorValue) = v2 /\ nth_def eff eff1 [] (S i) = eff'' /\ nth_def ids id 0 (S i) = id'')
+->
+(forall j : nat,
+     j < Datatypes.length vals0 ->
+     | env, nth_def ids0 id 0 j, nth j exps ErrorExp, nth_def eff5 eff1 [] j | -e>
+     | nth_def ids0 id 0 (S j), inl (nth j vals0 ErrorValue),
+     nth_def eff5 eff1 [] (S j) |)
+->
+| env, last ids0 id, nth (Datatypes.length vals0) exps ErrorExp,
+      last eff5 eff1 | -e> | id'', inr ex, eff3 |
+->
+  False.
+Proof.
+  intros. pose (P := firstn_eq eff5 exps vals vals0 _ _ _ _ _ _ _
+                                H H0 H1 H2 H3 H4 H5 H6 H7). inversion P.
+Qed.
+
+
+Lemma firstn_eq_rev {env : Environment} {eff : list SideEffectList} : 
+   forall (eff5 : list SideEffectList) (exps : list Expression) (vals vals0 : list Value) 
+          (eff1 : SideEffectList) (ids ids0 : list nat) (id : nat) (eff2 : SideEffectList) 
+          (id' : nat) (ex : Exception),
+(forall j : nat,
+     j < Datatypes.length vals ->
+     forall (v2 : Value + Exception) (eff'' : SideEffectList) (id'' : nat),
+     | env, nth_def ids id 0 j, nth j exps ErrorExp, nth_def eff eff1 [] j | -e> | id'', v2, eff'' | ->
+     inl (nth j vals ErrorValue) = v2 /\ nth_def eff eff1 [] (S j) = eff'' /\ nth_def ids id 0 (S j) = id'')
+->
+(forall i : nat,
+     i < Datatypes.length exps ->
+     | env, nth_def ids0 id 0 i, nth i exps ErrorExp, nth_def eff5 eff1 [] i | -e>
+     | nth_def ids0 id 0 (S i), inl (nth i vals0 ErrorValue),
+     nth_def eff5 eff1 [] (S i) |) ->
+(forall (v2 : Value + Exception) (eff'' : SideEffectList) (id'' : nat),
+        | env, last ids id, nth (Datatypes.length vals) exps ErrorExp,
+        last eff eff1 | -e> | id'', v2, eff'' | ->
+        inr ex = v2 /\ eff2 = eff'' /\ id' = id'')
+->
+Datatypes.length vals < Datatypes.length exps ->
+Datatypes.length eff = Datatypes.length vals ->
+Datatypes.length exps = Datatypes.length vals0 ->
+Datatypes.length exps = Datatypes.length eff5 ->
+length exps = length ids0 ->
+length ids = length vals
+->
+False.
+Proof.
+  induction eff.
+  * intros. apply eq_sym, length_zero_iff_nil in H3. subst.
+    apply length_zero_iff_nil in H7. subst.
+    pose (P := H0 0 H2).
+    pose (P2 := H1 _ _ _ P). inversion P2. congruence.
+  * intros. destruct eff5.
+    - inversion H5. rewrite H5 in H2. inversion H2.
+    - inversion H3. inversion H5.
+    (* first elements *)
+      assert (0 < length exps). { lia. } assert (0 < length vals). { lia. }
+      assert (S (Datatypes.length eff5) = Datatypes.length exps). { auto. }
+      assert (Datatypes.length exps = Datatypes.length vals0) as LENGTH. { auto. }
+      assert (S (Datatypes.length eff) = Datatypes.length vals) as Helper1. { auto. }
+      assert (Datatypes.length exps = Datatypes.length ids0) as Helper2. { auto. }
+      (* single_unfold_list H9. *)
+      pose (EE1 := element_exist (length eff5) exps (eq_sym H5)).
+      pose (EE2 := element_exist (length eff) vals H9).
+      rewrite H5 in H4, H6. rewrite <- H9 in H7.
+      pose (EE3 := element_exist (length eff5) vals0 H4).
+      pose (EE4 := element_exist _ _ (eq_sym H7)).
+      pose (EE5 := element_exist _ _ H6).
+      
+      inversion EE1 as [e]. inversion EE2 as [v]. inversion EE3 as [v'].
+      inversion EE4 as [id0']. inversion EE5 as [id0'']. 
+      inversion H13. inversion H14. inversion H15. inversion H16. inversion H17. subst.
+      pose (P0 := H0 0 H8).
+      pose (P1 := H 0 H11 (inl v') s).
+      pose (P2 := P1 _ P0). destruct P2. destruct H19. inversion H18. simpl in H19, H20. subst.
+    (* other elements *)
+      inversion H3.
+      apply IHeff with (exps := x) (vals := x0) (eff1 := s) (vals0 := x1)
+                  (ids := x2) (ids0 := x3) (id := id0'') (ex := ex) (eff5 := eff5)
+                  (eff2 := eff2) (id' := id'); auto.
+        + intros. assert (S j < Datatypes.length (v' :: x0)). { simpl. lia. } 
+          pose (A := H (S j) H22 v2 eff'').
+          pose (B := A _ H21). assumption.
+        + intros. assert (S i < Datatypes.length (e :: x)). { simpl. lia. } 
+          pose (A := H0 (S i) H21). exact A.
+        + intros. rewrite <- last_element_equal, <- last_element_equal in H1. apply H1. assumption.
+        + intuition.
+        + inversion H7. lia.
+Qed.
+
+(** First i (length vals) element are equal with concatn *)
+Lemma eff_until_i_rev {env : Environment} {eff : list SideEffectList} : 
+   forall (eff5 : list SideEffectList) (exps : list Expression) (vals vals0 : list Value) 
+          (eff1 : SideEffectList) (ids ids0 : list nat) (id : nat) (eff2 : SideEffectList) 
+          (id' : nat) (ex : Exception),
+(forall j : nat,
+     j < Datatypes.length vals ->
+     forall (v2 : Value + Exception) (eff'' : SideEffectList) (id'' : nat),
+     | env, nth_def ids id 0 j, nth j exps ErrorExp, nth_def eff eff1 [] j | -e> | id'', v2, eff'' | ->
+     inl (nth j vals ErrorValue) = v2 /\ nth_def eff eff1 [] (S j) = eff'' /\ nth_def ids id 0 (S j) = id'')
+->
+(forall i : nat,
+     i < Datatypes.length exps ->
+     | env, nth_def ids0 id 0 i, nth i exps ErrorExp, nth_def eff5 eff1 [] i | -e>
+     | nth_def ids0 id 0 (S i), inl (nth i vals0 ErrorValue),
+     nth_def eff5 eff1 [] (S i) |) ->
+(forall (v2 : Value + Exception) (eff'' : SideEffectList) (id'' : nat),
+        | env, last ids id, nth (Datatypes.length vals) exps ErrorExp,
+        last eff eff1 | -e> | id'', v2, eff'' | ->
+        inr ex = v2 /\ eff2 = eff'' /\ id' = id'')
+->
+Datatypes.length vals < Datatypes.length exps ->
+Datatypes.length eff = Datatypes.length vals ->
+Datatypes.length exps = Datatypes.length vals0 ->
+Datatypes.length exps = Datatypes.length eff5 ->
+length exps = length ids0 ->
+length ids = length vals
+->
+False.
+Proof.
+  intros. apply (firstn_eq_rev eff5 exps vals vals0 eff1 _ _ _ _ _ _
+                                   H H0 H1 H2 H3 H4 H5 H6 H7).
+Qed.
+
+Lemma con_n_equality {env : Environment} {eff : list SideEffectList} : 
+  forall (exps : list Expression) (vals vals0 : list Value) eff1 eff6 i i0 ids ids0 id eff3 id' ex,
+(forall j : nat,
+    j < i ->
+    forall (v2 : Value + Exception) (eff'' : SideEffectList) (id'' : nat),
+    | env, nth_def ids id 0 j, nth j exps ErrorExp, nth_def eff eff1 [] j | -e> | id'', v2, eff'' | ->
+    inl (nth j vals ErrorValue) = v2 /\ nth_def eff eff1 [] (S j) = eff'' /\ nth_def ids id 0 (S j) = id'')
+->
+(forall j : nat,
+     j < i0 ->
+     | env, nth_def ids0 id 0 j, nth j exps ErrorExp, nth_def eff6 eff1 [] j | -e>
+     | nth_def ids0 id 0 (S j), inl (nth j vals0 ErrorValue),
+     nth_def eff6 eff1 [] (S j) |)
+->
+(forall (v2 : Value + Exception) (eff'' : SideEffectList) (id'' : nat),
+     | env, last ids id, nth i exps ErrorExp, last eff eff1 | -e> | id'', v2, eff'' | ->
+     inr ex = v2 /\ eff3 = eff'' /\ id' = id'')
+->
+Datatypes.length eff = i ->
+i < Datatypes.length exps ->
+Datatypes.length vals = i ->
+Datatypes.length vals0 = i0 ->
+i0 < Datatypes.length exps ->
+Datatypes.length eff6 = i0 ->
+length ids = i ->
+length ids0 = i0 ->
+i < i0
+->
+False.
+Proof.
+  induction eff.
+  * intros. simpl in H1. subst. simpl in H10. pose (P := H0 0 H10).
+    simpl in H8, P. apply length_zero_iff_nil in H8. subst.
+    pose (P2 := H1 _ _ _ P). inversion P2. congruence.
+  * intros. inversion H2. simpl in H2. rewrite <- H2 in H4.
+    pose (EE1 := element_exist (length eff) vals (eq_sym H4)). 
+    inversion EE1 as [v]. inversion H12 as [vs]. destruct eff6.
+    - simpl in H7. subst. rewrite <- H7 in H10. inversion H10.
+    - subst. simpl. (* simpl_concatn_H IHeff. rewrite concatn_app, concatn_app. simpl_concatn. *)
+      simpl in H7. (* single_unfold_list H6. *) 
+      pose (EE2 := element_exist (length eff6) vals0 H7). inversion EE2. 
+      inversion H2.
+      pose (NE := nat_lt_zero _ _  H3). inversion NE.
+      pose (EE3 := element_exist x1 exps (eq_sym H13)). inversion EE3. inversion H14.
+      subst. 
+      pose (EE4 := element_exist _ _ (eq_sym H8)).
+      pose (EE5 := element_exist _ _ (eq_sym H9)).
+      inversion EE4 as [id0']. inversion EE5 as [id0''].
+      inversion H5. inversion H15. subst.
+      assert (s = a /\ id0' = id0''). {
+        subst.
+        assert (0 < Datatypes.length (x :: x0)). {  simpl. lia. }
+        pose (P := H0 0 H16).
+        assert (0 < S (Datatypes.length eff)). {  simpl. lia. }
+        pose (P2 := H 0 H17 (inl (nth 0 (x :: x0) ErrorValue)) (nth_def (s :: eff6) eff1 [] 1) _ P). 
+        inversion P2.
+        destruct H19. auto.
+      }
+      destruct H16. subst.
+      
+      eapply IHeff with (exps := x3) (vals := vs) (vals0 := x0) (eff1 := a)
+                        (i0 := length x0) (ids := x4) (ids0 := x5); auto.
+      + intros. assert (S j < S (Datatypes.length eff)). { simpl. lia. }
+        pose (P := H (S j) H18 v2 eff'' id''). pose (P H17). assumption.
+      + intros. assert (S j < Datatypes.length (x :: x0)). { simpl. lia. }
+        pose (P := H0 (S j) H17). exact P.
+      + intros. apply H1.
+        rewrite (last_element_equal _ _ id), (last_element_equal _ _ eff1) in H16.
+        exact H16.
+      + intuition.
+      + intuition.
+      + intuition.
+      + intuition.
+Qed.
+
+Lemma con_n_equality_rev {env : Environment} {eff : list SideEffectList} : 
+forall (exps : list Expression) (vals vals0 : list Value) (eff1 : SideEffectList) 
+   (eff6 : list SideEffectList) (i i0 : nat) (id : nat) (ids ids0 : list nat) id' ex0 eff4,
+(forall j : nat,
+    j < i ->
+    forall (v2 : Value + Exception) (eff'' : SideEffectList) (id'' : nat),
+    | env, nth_def ids id 0 j, nth j exps ErrorExp, nth_def eff eff1 [] j | -e> | id'', v2, eff'' | ->
+    inl (nth j vals ErrorValue) = v2 /\ nth_def eff eff1 [] (S j) = eff'' /\ nth_def ids id 0 (S j) = id'')
+->
+(forall j : nat,
+     j < i0 ->
+     | env, nth_def ids0 id 0 j, nth j exps ErrorExp, nth_def eff6 eff1 [] j | -e> 
+     | nth_def ids0 id 0 (S j), inl (nth j vals0 ErrorValue),
+     nth_def eff6 eff1 [] (S j) |)
+->
+Datatypes.length eff = i ->
+i < Datatypes.length exps ->
+Datatypes.length vals = i ->
+Datatypes.length vals0 = i0 ->
+i0 < Datatypes.length exps ->
+Datatypes.length eff6 = i0 ->
+length ids = i ->
+length ids0 = i0 ->
+i > i0 ->
+(| env, last ids0 id, nth i0 exps ErrorExp, last eff6 eff1 | -e> | id', 
+     inr ex0,eff4 |)
+->
+False.
+Proof.
+induction eff.
+  * intros. simpl in H1. subst. inversion H9.
+  * intros. simpl in H1. rewrite <- H1 in H3.
+    pose (EE1 := element_exist (length eff) vals (eq_sym H3)).
+    inversion EE1 as [v]. inversion H11 as [vs]. destruct eff6.
+    - subst. apply eq_sym, length_zero_iff_nil in H6. subst. apply length_zero_iff_nil in H8.
+      subst.
+      simpl in H10. pose (P := H 0 (Nat.lt_0_succ _) _ _ _ H10). inversion P. congruence.
+    - subst.
+      assert (Datatypes.length ids0 = Datatypes.length vals0) as Helper. { auto. }
+      pose (EE2 := element_exist (length eff6) vals0 H6). inversion EE2. inversion H1.
+      pose (NE := nat_lt_zero _ _ H2). inversion NE.
+      pose (EE3 := element_exist x1 exps (eq_sym H12)). inversion EE3.
+      inversion H13. subst.
+      pose (EE4 := element_exist _ _ (eq_sym H7)).
+      pose (EE5 := element_exist _ _ (eq_sym H8)).
+      inversion EE4 as [id0']. inversion EE5 as [id0'']. inversion H4. inversion H14. subst.
+      assert (s = a /\ id0' = id0''). {
+        subst.
+        assert (0 < Datatypes.length (x :: x0)). {  simpl. lia. }
+        pose (P := H0 0 H15).
+        assert (0 < S (Datatypes.length eff)). {  simpl. lia. }
+        pose (P1 := H 0 H16 (inl (nth 0 (x :: x0) ErrorValue)) (nth_def (s :: eff6) eff1 [] 1) _ P).
+        destruct P1. destruct H18. simpl in H19, H18. auto.
+      }
+      destruct H15. subst.
+      eapply IHeff with (exps := x3) (vals := vs) (vals0 := x0) (eff1 := a) 
+                       (i0 := length eff6) (i := length eff) (ids := x4) (ids0 := x5); auto.
+      + intros. assert (S j < S (Datatypes.length eff)). { simpl. lia. }
+        pose (P := H (S j) H17 v2 eff''). simpl in P.
+        pose (P1 := P _ H16). assumption.
+      + intros. inversion H6. assert (S j < Datatypes.length (x :: x0)). { simpl. lia. }
+        pose (P := H0 (S j) H16). assumption.
+      + intuition.
+      + inversion H6. auto.
+      + rewrite <- H6 in H5. simpl in H5. lia.
+      + rewrite <- H6 in Helper. auto.
+      + simpl in *. rewrite <- H6 in H9. lia.
+      + rewrite <- last_element_equal, <- last_element_equal in H10. simpl in H10. 
+        inversion H6. rewrite H16. exact H10.
+Qed.
+
+
+Lemma list_equal_until_i {env : Environment} {eff : list SideEffectList} :
+  forall (exps : list Expression) (vals vals0 : list Value) (eff6 : list SideEffectList)
+      (eff1 : SideEffectList) (ids ids0 : list nat) (id : nat),
+(forall j : nat,
+    j < Datatypes.length vals ->
+    forall (v2 : Value + Exception) (eff'' : SideEffectList) (id'' : nat),
+    | env, nth_def ids id 0 j, nth j exps ErrorExp, nth_def eff eff1 [] j | -e> | id'', v2, eff'' | ->
+    inl (nth j vals ErrorValue) = v2 /\ nth_def eff eff1 [] (S j) = eff'' /\ nth_def ids id 0 (S j) = id'')
+->
+(forall j : nat,
+     j < Datatypes.length vals0 ->
+     | env, nth_def ids0 id 0 j, nth j exps ErrorExp, nth_def eff6 eff1 [] j | -e> 
+     | nth_def ids0 id 0 (S j), inl (nth j vals0 ErrorValue),
+     nth_def eff6 eff1 [] (S j) |)
+->
+Datatypes.length vals = Datatypes.length vals0
+->
+Datatypes.length eff = Datatypes.length vals
+->
+Datatypes.length eff6 = Datatypes.length vals0
+->
+Datatypes.length vals0 < Datatypes.length exps
+->
+length ids = length vals
+->
+length ids0 = length vals0
+->
+eff = eff6 /\ vals = vals0 /\ ids = ids0.
+Proof.
+  induction eff.
+  * intros. inversion H2. apply eq_sym, length_zero_iff_nil in H8. subst. simpl in H1. 
+    apply eq_sym, length_zero_iff_nil in H1. subst. simpl in H3. apply length_zero_iff_nil in H3. 
+    apply length_zero_iff_nil in H5. apply length_zero_iff_nil in H6. subst. auto.
+  * intros. simpl in H2. rewrite <- H2 in H1. rewrite <- H1 in H3. pose (NE := nat_lt_zero _ _ H4). inversion NE.
+    (* single_unfold_list H2. *)
+    pose (EE1 := element_exist (length eff) vals H2).
+    pose (EE2 := element_exist (length eff) vals0 H1).
+    pose (EE3 := element_exist (length eff) eff6 (eq_sym H3)).
+    pose (EE4 := element_exist x exps (eq_sym H7)).
+    inversion EE1 as [v]. inversion EE2 as [v']. inversion EE3 as [fe]. inversion EE4 as [e'].
+    inversion H8. inversion H9. inversion H10. inversion H11. subst.
+    pose (EE5 := element_exist _ _ (eq_sym H5)).
+    pose (EE6 := element_exist _ _ (eq_sym H6)).
+    inversion EE5 as [id']. inversion EE6 as [id''].
+    inversion H12. inversion H13. subst.
+    assert (0 < Datatypes.length (v' :: x1)). { simpl. lia. }
+    pose (P := H0 0 H14).
+    assert (0 < Datatypes.length (v :: x0)). { simpl. lia. }
+    pose (P1 := H 0 H15 (inl (nth 0 (v' :: x1) ErrorValue)) (nth_def (fe :: x2) eff1 [] 1) _ P).
+    inversion P1. destruct H17. simpl in H18. inversion H16. simpl in H17. subst.
+    
+    assert (eff = x2 /\ x0 = x1 /\ x4 = x5).
+    {
+      apply IHeff with (exps := x3) (vals := x0) (vals0 := x1) (eff1 := fe) (id := id''); auto.
+      + intros. assert (S j < S (Datatypes.length x0)). { simpl. lia. } pose (P2 := H (S j) H19 v2 eff''). 
+        simpl in P2. pose (P2 _ H18). assumption.
+      + intros. assert (S j < Datatypes.length (v' :: x1)). { simpl. lia. }
+        pose (P3 := H0 (S j) H18). simpl in P3. assumption.
+      + inversion H2. inversion H3. inversion H1. auto.
+      + inversion H2. inversion H3. inversion H1. auto.
+      + intuition.
+    }
+    inversion H17. inversion H19. subst. auto.
+Qed.
+
+Lemma exception_equality {env : Environment} {exps : list Expression} (vals vals0 : list Value) 
+   (ex : Exception) (eff1 : SideEffectList) (eff eff6 : list SideEffectList) (i i0 : nat) 
+   (eff3 : SideEffectList) (ex0 : Exception) (eff4 : SideEffectList) (ids ids0 : list nat)
+   (id id' id'' : nat) :
+(forall j : nat,
+     j < i ->
+     forall (v2 : Value + Exception) (eff'' : SideEffectList) (id'' : nat),
+     | env, nth_def ids id 0 j, nth j exps ErrorExp, nth_def eff eff1 [] j | -e> | id'', v2, eff'' | ->
+     inl (nth j vals ErrorValue) = v2 /\ nth_def eff eff1 [] (S j) = eff'' /\ nth_def ids id 0 (S j) = id'')
+->
+| env, last ids0 id, nth i0 exps ErrorExp, last eff6 eff1 | -e>
+| id'', inr ex0, eff4 |
+->
+(forall (v2 : Value + Exception) (eff'' : SideEffectList) (id'' : nat),
+        | env, last ids id, nth i exps ErrorExp, last eff eff1 | -e>
+        | id'', v2, eff'' | -> inr ex = v2 /\ eff3 = eff'' /\ id' = id'')
+->
+(forall j : nat,
+      j < i0 ->
+      | env, nth_def ids0 id 0 j, nth j exps ErrorExp, nth_def eff6 eff1 [] j | -e>
+      | nth_def ids0 id 0 (S j), inl (nth j vals0 ErrorValue),
+      nth_def eff6 eff1 [] (S j) |)
+->
+Datatypes.length vals = i ->
+ i < Datatypes.length exps ->
+ Datatypes.length eff = i ->
+ Datatypes.length vals0 = i0 ->
+ i0 < Datatypes.length exps ->
+ Datatypes.length eff6 = i0 ->
+ length ids = i ->
+ length ids0 = i0
+->
+i = i0 /\ eff = eff6 /\ vals = vals0 /\ ids = ids0.
+Proof.
+  intros.
+  destruct (Compare_dec.le_gt_dec i i0).
+  * case_eq (Lt.le_lt_or_eq i i0 l).
+    - intros.
+      pose (P1 := con_n_equality exps vals vals0 eff1 eff6 i i0 ids ids0 id _ _ _
+                 H H2 H1 H5 H4 H3 H6 H7 H8 H9 H10 l0). inversion P1.
+    - intros. subst. pose (list_equal_until_i exps vals vals0 eff6 eff1 _ _ _
+                            H H2 e H5 H8 H7 H9 H10). auto.
+  * pose (P := con_n_equality_rev exps vals vals0 eff1 eff6 i i0 id ids ids0 _ _ _
+               H H2 H5 H4 H3 H6 H7 H8 H9 H10 g H0). inversion P.
+Qed.
+
+Theorem determinism : forall {env : Environment} {e : Expression} {v1 : Value + Exception} 
+    {id id' : nat} {eff eff' : SideEffectList}, 
+  |env, id, e, eff| -e> | id', v1, eff'|
+->
+  (forall v2 eff'' id'', |env, id, e, eff| -e> |id'', v2, eff''| -> v1 = v2 /\ eff' = eff''
+      /\ id' = id'').
+Proof.
+  intro. intro. intro. intro. intro. intro. intro. intro IND. induction IND.
+  (* LITERAL, VARIABLE, FUNCTION SIGNATURE, FUNCTION DEFINITION *)
+  1-4: intros; inversion H; try(inversion H0); subst; auto.
+  * intros. inversion H. auto.
+
+  (* CALL *)
+  * intros. inversion H6.
+    - subst.
+      pose (LEQ := list_equality vals vals0 eff eff4 _ _ _ H2 H3 H12 H9 H10 H H0 H1 H11).
+      destruct LEQ. destruct H7. subst. rewrite H4 in H15. inversion H15.
+      subst. auto.
+    - subst. pose (P1 := H3 (Datatypes.length vals0) H9 (inr ex)
+                            eff'').
+      pose (EU := @eff_until_i env eff eff4 params vals vals0 eff1 _ _ id _ _ _ 
+                H H0 H11 H9 H1 H12 H3 H15 H20). inversion EU.
+
+  (* APPLY *)
+  * intros. inversion H5.
+    - subst. apply IHIND1 in H9. inversion H9. destruct H7.
+      inversion H6. subst.
+      pose (EQ := list_equality vals vals0 eff eff6 _ _ _ H3 H4 H15 H8 H11 H H1 H2 H12).
+      inversion EQ. destruct H13. subst.
+      apply IHIND2 in H20. destruct H20. destruct H13. auto.
+    - subst. apply IHIND1 in H14. inversion H14. congruence.
+    - subst. apply IHIND1 in H12. destruct H12. destruct H7.
+      inversion H6. subst.
+      pose (P1 := @eff_until_i env eff eff6 params vals vals0 _ _ _ _ _ _ _
+                H H1 H10 H8 H2 H11 H4 H15 H20).
+      inversion P1.
+    - subst. apply IHIND1 in H11. inversion H11. inversion H6. subst.
+      pose (P := H13 ref ext var_list body). congruence.
+    - subst. apply IHIND1 in H11. inversion H11. inversion H6. subst. congruence.
+
+  (* LET *)
+  * intros. inversion H; subst.
+    - apply IHIND1 in H9. destruct H9, H1. inversion H0. subst.
+      apply IHIND2. auto.
+    - apply IHIND1 in H9. destruct H9. congruence.
+
+  (* LETREC *)
+  * intros. inversion H. 
+    - subst. apply IHIND. auto.
+
+  (* CORECT TRY *)
+  * intros. inversion H; subst.
+    - apply IHIND1 in H11. destruct H11, H1. inversion H0. subst.
+      apply IHIND2. auto.
+    - apply IHIND1 in H11. destruct H11. congruence.
+
+  (* CORRECT CATCH *)
+  * intros. inversion H; subst.
+    - apply IHIND1 in H11. destruct H11, H1. inversion H0.
+    - apply IHIND1 in H11. destruct H11, H1. inversion H0. subst. apply IHIND2. auto.
+
+  (* CALL EXCEPTION *)
+  * intros. inversion H5.
+    - subst.
+      pose (EU := @eff_until_i_rev env eff _ params vals vals0 eff1 ids ids0 id _ _ _
+              H4 H11 IHIND H H1 H8 H9 H10 H2). inversion EU.
+    - apply IHIND.
+      pose (EEQ := exception_equality vals vals0 ex eff1 eff _ i
+             i0 _ ex0 _ _ _ _ _ _ H4 H19 IHIND H14 H0 H H1 H9 H8 H10 H2 H11).
+      destruct EEQ. destruct H21. destruct H22. subst. assumption.
+
+  (* APPLY EXCEPTION *)
+  (* name evaluates to an exception *)
+  * intros. inversion H.
+    - subst. pose (IH := IHIND _ _ _ H3). inversion IH. congruence.
+    - subst. apply IHIND. assumption.
+    - subst. pose (IH := IHIND _ _ _ H6). inversion IH. congruence.
+    - subst. pose (IH := IHIND _ _ _ H5). inversion IH. congruence.
+    - subst. pose (IH := IHIND _ _ _ H5). inversion IH. congruence.
+
+  (* parameter exception *)
+  * intros. inversion H5.
+    - subst. apply IHIND1 in H9. destruct H9. destruct H6. inversion H0.
+      subst.
+      pose (P1 := @eff_until_i_rev env eff _ params vals vals0 _ ids ids0 id'0 _ _ _
+                   H4 H15 IHIND2 H H1 H8 H11 H12 H2). inversion P1.
+    - subst. apply IHIND1 in H14. inversion H14. congruence.
+    - apply IHIND1 in H12. destruct H12. destruct H21. inversion H12.
+      rewrite H21, H22, H24 in *.
+      assert (| env, last ids0 id'0, nth i0 params ErrorExp, last eff6 eff4 | -e> | id''0, inr ex0, eff'' |). { assumption. }
+      pose (EE := exception_equality vals vals0 ex _ eff _ i i0 _ ex0
+                 _ _ _ _ _ _ H4 H20 IHIND2 H15 H0 H H1 H9 H8 H10 H2 H11).
+      destruct EE. destruct H26. destruct H27. subst.
+      apply IHIND2 in H23.
+      assumption.
+    - subst. apply IHIND1 in H11. destruct H11. inversion H0. destruct H6.
+      subst.
+      pose (P1 := @eff_until_i_rev env eff _ params vals vals0 _ ids ids0 id'0 _ _ _
+                 H4 H12 IHIND2 H H1 H8 H9 H10 H2). inversion P1.
+    - subst. apply IHIND1 in H11. destruct H11. inversion H0. destruct H6.
+      subst.
+      pose (P1 := @eff_until_i_rev env eff _ params vals vals0 _ ids ids0 id'0 _ _ _
+                 H4 H12 IHIND2 H H1 H8 H9 H10 H2). inversion P1.
+
+  (* name evaluate to a non-closure value *)
+  * intros. inversion H7.
+    - apply IHIND in H11. destruct H11. destruct H23. inversion H11.
+      pose (P := H4 ref ext var_list body _ H26). inversion P.
+    - subst. apply IHIND in H16. inversion H16. congruence.
+    - subst. apply IHIND in H14. destruct H14. inversion H5. destruct H6.
+      subst.
+      pose (P1 := @eff_until_i env eff _ params vals vals0 _ ids ids0 id'0 id''0 ex _
+                         H H0 H12 H10 H1 H13 H3 H17 H22). inversion P1.
+    - subst. apply IHIND in H13. destruct H13. inversion H5. destruct H6. subst.
+      pose (LEQ := @list_equality env params _ vals vals0 eff _ _ _ _
+                     H2 H3 H14 H10 H11 H H0 H1 H12).
+      destruct LEQ. destruct H8. subst. auto.
+    - subst. apply IHIND in H13. destruct H13. inversion H5. destruct H6. subst.
+      pose (P := H4 ref ext var_list body). congruence.
+
+  (* paramlist is too short/long *)
+  * intros. inversion H7.
+    - subst. 
+      pose (P1 := IHIND _ _ _ H11). destruct P1. destruct H6. inversion H5. subst.
+      pose (EL:= list_equality vals vals0 eff _ _ _ _ H2 H3 H17 H10 H13 H H0 H1 H14).
+      destruct EL. destruct H8. subst. intuition. 
+    - subst. pose (IH := IHIND _ _ _ H16). inversion IH. congruence.
+    - subst.
+      pose (P1 := IHIND _ _ _ H14). destruct P1. destruct H6. inversion H5. subst.
+      pose (P2 := @eff_until_i env eff _ params vals vals0 _ ids ids0 id'0 id''0 ex _
+                     H H0 H12 H10 H1 H13 H3 H17 H22). inversion P2.
+    - subst.
+      pose (P1 := IHIND _ _ _ H13). destruct P1. destruct H6. inversion H5. subst.
+      pose (P2 := H15 ref ext var_list body).
+      congruence.
+    - subst.
+      pose (P1 := IHIND _ _ _ H13). destruct P1. destruct H6. inversion H5. subst.
+      pose (EL:= list_equality vals vals0 eff _ _ _ _ H2 H3 H14 H10 H11 H H0 H1 H12).
+      destruct EL. destruct H8. subst. auto.
+
+  
+  (* LET EXCEPTION *)
+  * intros. inversion H; subst.
+    - apply IHIND in H9. destruct H9. congruence.
+    - apply IHIND in H9. destruct H9. destruct H1. inversion H0. auto.
+Qed.
+
+
+
+End determinism_proof.
+
+
